almost done w correctness finished minheap correctness just refactoring the meld one

Thesis/pqueue.lean
@@ -1,6 +1,7 @@
 import Lean
 import Mathlib.Tactic
 
+-- Leftist heap definition and methods
 inductive leftistHeap (β : Type) where
 | leaf
 | node (left : leftistHeap β) (key : β) (priority : Int) (rank : Nat) (right : leftistHeap β)
@@ -32,6 +33,12 @@ def meld {β : Type} : leftistHeap β → leftistHeap β → leftistHeap β
 def insertLeftist {β : Type} (h : leftistHeap β) (key : β) (priority : Int) : leftistHeap β :=
   meld h (singleton key priority)
 
+def deleteMinLeftist {β : Type} (h : leftistHeap β) : Option β × leftistHeap β :=
+  match h with
+  | leaf => (none, leaf)
+  | node left key _ _ right => (key, meld left right)
+
+-- ForAllHeap predicate and lemmas
 inductive forAllHeap {β : Type} (p : β → Int → Prop) : leftistHeap β → Prop
 | leaf : forAllHeap p leaf
 | node left key priority rank right :
@@ -40,126 +47,255 @@ inductive forAllHeap {β : Type} (p : β → Int → Prop) : leftistHeap β → 
     forAllHeap p right →
     forAllHeap p (node left key priority rank right)
 
-theorem parentPredicate : ∀ (β : Type) (p : β → Int → Prop) (left right : leftistHeap β) (key : β) (priority : Int) (rank : Nat),
+lemma parentPredicate : ∀ (β : Type) (p : β → Int → Prop) (left right : leftistHeap β) (key : β) (priority : Int) (rank : Nat),
   forAllHeap p (node left key priority rank right) → p key priority := by
-  intro β p left right key priority rank h
-  rcases h with ⟨h1, h2, h3⟩
-  trivial
+    intro β p left right key priority rank h
+    rcases h with ⟨h1, h2, h3⟩
+    trivial
 
-theorem leftForAllHeap : ∀ (β : Type) (p : β → Int → Prop) (left right : leftistHeap β) (key : β) (priority : Int) (rank : Nat),
+lemma leftForAllHeap : ∀ (β : Type) (p : β → Int → Prop) (left right : leftistHeap β) (key : β) (priority : Int) (rank : Nat),
   forAllHeap p (node left key priority rank right) → forAllHeap p left := by
-  intro β p left right key priority rank h
-  rcases h with ⟨h1, h2, h3⟩
-  trivial
+    intro β p left right key priority rank h
+    rcases h with ⟨h1, h2, h3⟩
+    trivial
 
-theorem rightForAllHeap : ∀ (β : Type) (p : β → Int → Prop) (left right : leftistHeap β) (key : β) (priority : Int) (rank : Nat),
+lemma rightForAllHeap : ∀ (β : Type) (p : β → Int → Prop) (left right : leftistHeap β) (key : β) (priority : Int) (rank : Nat),
   forAllHeap p (node left key priority rank right) → forAllHeap p right := by
-  intro β p left right key priority rank h
-  rcases h with ⟨h1, h2, h3⟩
-  trivial
+    intro β p left right key priority rank h
+    rcases h with ⟨h1, h2, h3⟩
+    trivial
 
-theorem forAllHeap_insertLeftist : ∀ (β : Type) (p : β → Int → Prop) (h : leftistHeap β),
-  forAllHeap p h →
-    ∀(newKey : β) (newPriority : Int), p newKey newPriority →
-      forAllHeap p (insertLeftist h newKey newPriority) := by
-
-  intro β p h hP newKey newPriority pNew
-  induction h with
-  | leaf =>
-      rw [insertLeftist, meld, singleton]
+theorem leftLessThanHeap : ∀ (β : Type) (left right : leftistHeap β) (key : β) (priority newPriority : Int) (rank : Nat),
+  forAllHeap (fun _ p => priority ≤ p) (node left key priority rank right) → newPriority ≤ priority → forAllHeap (fun _ pL => newPriority ≤ pL) left := by
+  intro β left right key priority newPriority rank h hPP
+  induction left with
+  | leaf => apply forAllHeap.leaf
+  | node lLeft lKey lPriority lRank lRight ihL ihR =>
+      have lol : forAllHeap (fun _ pL => priority ≤ pL) (node lLeft lKey lPriority lRank lRight) :=
+          leftForAllHeap β (fun _ pL => priority ≤ pL) (node lLeft lKey lPriority lRank lRight) right key priority rank h
+      have lol' : priority ≤ lPriority := parentPredicate β _ lLeft lRight lKey lPriority lRank lol
       apply forAllHeap.node
-      apply pNew
-      apply forAllHeap.leaf
-      apply forAllHeap.leaf
+      . apply le_trans
+        . apply hPP
+        . apply lol'
+      . apply ihL
+        . apply forAllHeap.node
+          . trivial
+          . apply leftForAllHeap β (fun _ pL => priority ≤ pL) lLeft lRight lKey lPriority lRank lol
+          . exact rightForAllHeap β (fun _ pL => priority ≤ pL) (node lLeft lKey lPriority lRank lRight) right key priority rank h
+      . apply ihR
+        . apply forAllHeap.node
+          . trivial
+          . exact rightForAllHeap β (fun _ pL => priority ≤ pL) lLeft lRight lKey lPriority lRank lol
+          . exact rightForAllHeap β (fun _ pL => priority ≤ pL) (node lLeft lKey lPriority lRank lRight) right key priority rank h
 
-  | node left key priority rank right ihL ihR =>
-      rw [insertLeftist, meld.eq_def, singleton]
+-- theorem forAllHeap_insertLeftist : ∀ (β : Type) (p : β → Int → Prop) (h : leftistHeap β),
+  -- forAllHeap p h →
+  -- ∀(newKey : β) (newPriority : Int), p newKey newPriority →
+  -- forAllHeap p (insertLeftist h newKey newPriority) := by
+
+  -- intro β p h hP newKey newPriority pNew
+  -- induction h with
+  -- | leaf =>
+  --     rw [insertLeftist, meld, singleton]
+  --     apply forAllHeap.node
+  --     apply pNew
+  --     apply forAllHeap.leaf
+  --     apply forAllHeap.leaf
+
+  -- | node left key priority rank right ihL ihR =>
+  --     rw [insertLeftist, meld.eq_def, singleton]
+  --     simp
+  --     split
+  --     case isTrue hPP =>
+  --       rw [mkLeftistNode]
+  --       split
+  --       case isTrue =>
+  --         apply leftistHeap.forAllHeap.node
+  --         . apply parentPredicate β p left right key priority rank hP
+  --         . rw [insertLeftist, singleton] at ihR
+  --           apply ihR
+  --           apply rightForAllHeap β p left right key priority rank hP
+  --         . apply leftForAllHeap β p left right key priority rank hP
+  --       case isFalse =>
+  --         apply leftistHeap.forAllHeap.node
+  --         . apply parentPredicate β p left right key priority rank hP
+  --         . apply leftForAllHeap β p left right key priority rank hP
+  --         . rw [insertLeftist, singleton] at ihR
+  --           apply ihR
+  --           apply rightForAllHeap β p left right key priority rank hP
+
+  --     case isFalse hPP =>
+  --       rw [mkLeftistNode]
+  --       split
+  --       case isTrue =>
+  --         rw [meld.eq_def]
+  --         simp
+  --         apply forAllHeap.node
+  --         apply pNew
+  --         apply hP
+  --         exact forAllHeap.leaf
+  --       case isFalse =>
+  --         rw [meld.eq_def]
+  --         simp
+  --         apply forAllHeap.node
+  --         apply pNew
+  --         apply forAllHeap.leaf
+  --         exact hP
+
+def mkLeftistForAll : ∀ (β : Type) (p : β → Int → Prop) (left right : leftistHeap β) (key : β) (priority : Int),
+  forAllHeap p (mkLeftistNode left key priority right) →
+  forAllHeap p left ∧ forAllHeap p right := by
+    intro β p left right key priority h
+    rw [mkLeftistNode] at h
+    split at h
+    . constructor
+      . exact rightForAllHeap β p right left key priority ((left.rank) + 1) h
+      . exact leftForAllHeap β p right left key priority ((left.rank) + 1) h
+    . constructor
+      . exact leftForAllHeap β p left right key priority ((right.rank) + 1) h
+      . exact rightForAllHeap β p left right key priority ((right.rank) + 1) h
+
+def meldForAllHeap : ∀ (β : Type) (priority : Int) (a b : leftistHeap β),
+  forAllHeap (fun _ pA ↦ priority ≤ pA) a → forAllHeap (fun _ pB ↦ priority ≤ pB) b → forAllHeap (fun _ pAB ↦ priority ≤ pAB) (meld a b) := by
+  intro β priority a b hA hB
+  induction a with
+  | leaf =>
+      rw [meld.eq_def]
       simp
-      split
-      case isTrue hPP =>
-        rw [mkLeftistNode]
-        split
-        case isTrue =>
-          apply leftistHeap.forAllHeap.node
-          . apply parentPredicate β p left right key priority rank hP
-          . rw [insertLeftist, singleton] at ihR
-            apply ihR
-            apply rightForAllHeap β p left right key priority rank hP
-          . apply leftForAllHeap β p left right key priority rank hP
-        case isFalse =>
-          apply leftistHeap.forAllHeap.node
-          . apply parentPredicate β p left right key priority rank hP
-          . apply leftForAllHeap β p left right key priority rank hP
-          . rw [insertLeftist, singleton] at ihR
-            apply ihR
-            apply rightForAllHeap β p left right key priority rank hP
-
-      case isFalse hPP =>
-        rw [mkLeftistNode]
-        split
-        case isTrue =>
+      exact hB
+  | node la ka pa rka ra ihLa ihRa =>
+      induction b with
+      | leaf =>
           rw [meld.eq_def]
           simp
-          apply forAllHeap.node
-          apply pNew
-          apply hP
-          exact forAllHeap.leaf
-        case isFalse =>
+          exact hA
+      | node lb kb pb rkb rb ihLb ihRb =>
           rw [meld.eq_def]
           simp
-          apply forAllHeap.node
-          apply pNew
-          apply forAllHeap.leaf
-          exact hP
+          split_ifs with hle
+          . rw [mkLeftistNode]
+            split
+            . apply forAllHeap.node
+              . apply parentPredicate β (fun _ pA ↦ priority ≤ pA) la ra ka pa rka hA
+              . apply ihRa
+                exact rightForAllHeap β (fun _ pA ↦ priority ≤ pA) la ra ka pa rka hA
+              . apply leftForAllHeap β (fun _ pA ↦ priority ≤ pA) la ra ka pa rka hA
 
--- def meldForAllHeap : ∀ (β : Type) (p : β → Int → Prop) (a b : leftistHeap β), forAllHeap p a → forAllHeap p b → forAllHeap p (meld a b) := by
---   intro β p a b hA hB
---   induction a with
---   | leaf =>
---       rw [meld]
---       exact hB
---   | node la ka pa rka ra ihLa ihRa =>
---       induction b with
---       | leaf =>
---           rw [meld]
---           exact hA
---           intro _
---           trivial
+            . apply forAllHeap.node
+              . apply parentPredicate β (fun _ pA ↦ priority ≤ pA) la ra ka pa rka hA
+              . apply leftForAllHeap β (fun _ pA ↦ priority ≤ pA) la ra ka pa rka hA
+              . apply ihRa
+                exact rightForAllHeap β (fun _ pA ↦ priority ≤ pA) la ra ka pa rka hA
+          . rw [mkLeftistNode]
+            rw [not_lt] at hle
+            split
+            . apply forAllHeap.node
+              . apply parentPredicate β (fun _ pB ↦ priority ≤ pB) lb rb kb pb rkb hB
+              . apply ihRb
+                . apply rightForAllHeap β (fun _ pB ↦ priority ≤ pB) lb rb kb pb rkb hB
+                . intro hLa
+                  have hlB : forAllHeap (fun _ pB ↦ priority ≤ pB) (la.meld (lb.node kb pb rkb rb)) := by apply ihLa hLa
+                  have hrB : forAllHeap (fun _ pB ↦ priority ≤ pB) rb := by apply rightForAllHeap β (fun _ pB ↦ priority ≤ pB) lb rb kb pb rkb hB
+                  rw [meld.eq_def] at hlB
+                  cases la with
+                  | leaf =>
+                      rw [meld.eq_def]
+                      simp
+                      exact hrB
+                  | node lla kla pla rkla rla =>
+                      have lP
+                      have lPriority : ¬ pla < pb := by
+                        rw [not_lt]
+                        apply le_trans
+                        . apply hle
+                        . have lol : forAllHeap (fun _ pL ↦ pa ≤ pL) (node lla kla pla rkla rla) := by
+                            apply leftForAllHeap β (fun _ pA ↦ pa ≤ pA) (node lla kla pla rkla rla) ra ka pa rka
 
---       | node lb kb pb rkb rb ihLb ihRb =>
---           rw [meld, mkLeftistNode, mkLeftistNode]
---           split
---           . split
---             . apply forAllHeap.node
---               apply parentPredicate β p la ra ka pa rka hA
---               apply ihRa
---               apply rightForAllHeap β p la ra ka pa rka hA
---               apply leftForAllHeap β p la ra ka pa rka hA
+                          apply parentPredicate β (fun _ pA ↦ pa ≤ pA) lla rla kla pla rkla lol
+                      simp [lPriority] at hlB
+                      have bothForAll : forAllHeap (fun _ pB ↦ priority ≤ pB) lb ∧ forAllHeap (fun _ pB ↦ priority ≤ pB) ((lla.node kla pla rkla rla).meld rb) := by
+                        apply mkLeftistForAll β (fun _ pB ↦ priority ≤ pB) lb ((lla.node kla pla rkla rla).meld rb) kb pb hlB
+                      exact bothForAll.right
+                . sorry
+              . apply leftForAllHeap β (fun _ pA ↦ priority ≤ pA) lb rb kb pb rkb hB
+            . sorry
 
---             . apply forAllHeap.node
---               apply parentPredicate β p la ra ka pa rka hA
---               apply leftForAllHeap β p la ra ka pa rka hA
---               apply ihRa
---               apply rightForAllHeap β p la ra ka pa rka hA
+-- def meldForAllHeap : ∀ (β : Type) (p : β → Int → Prop) (a b : leftistHeap β),
+--   forAllHeap p a → forAllHeap p b → forAllHeap p (meld a b) := by
+--     intro β p a b hA hB
+--     induction a with
+--     | leaf =>
+--         rw [meld.eq_def]
+--         simp
+--         exact hB
+--     | node la ka pa rka ra ihLa ihRa =>
+--         induction b with
+--         | leaf =>
+--             rw [meld.eq_def]
+--             simp
+--             exact hA
+--         | node lb kb pb rkb rb ihLb ihRb =>
+--             rw [meld.eq_def]
+--             simp
+--             split_ifs with hle
+--             . rw [mkLeftistNode]
+--               split
+--               . apply forAllHeap.node
+--                 . apply parentPredicate β p la ra ka pa rka hA
+--                 . apply ihRa
+--                   exact rightForAllHeap β p la ra ka pa rka hA
+--                 . apply leftForAllHeap β p la ra ka pa rka hA
 
---           . split
---             . apply forAllHeap.node
---               apply parentPredicate β p lb rb kb pb rkb hB
---               apply ihRb
---               apply rightForAllHeap β p lb rb kb pb rkb hB
---               sorry
---               sorry
---               sorry
+--               . apply forAllHeap.node
+--                 . apply parentPredicate β p la ra ka pa rka hA
+--                 . apply leftForAllHeap β p la ra ka pa rka hA
+--                 . apply ihRa
+--                   exact rightForAllHeap β p la ra ka pa rka hA
 
---             . apply forAllHeap.node
---               apply parentPredicate β p lb rb kb pb rkb hB
---               apply leftForAllHeap β p lb rb kb pb rkb hB
---               apply ihRb
---               apply rightForAllHeap β p lb rb kb pb rkb hB
---               intro _
+--             . rw [mkLeftistNode]
+--               rw [not_lt] at hle
+--               split
+--               . apply forAllHeap.node
+--                 . apply parentPredicate β p lb rb kb pb rkb hB
+--                 . apply ihRb
+--                   . apply rightForAllHeap β p lb rb kb pb rkb hB
+--                   . intro hLa
+--                     have hlB : forAllHeap p (la.meld (lb.node kb pb rkb rb)) := by apply ihLa hLa
+--                     have hrB : forAllHeap p rb := by apply rightForAllHeap β p lb rb kb pb rkb hB
+--                     rw [meld.eq_def] at hlB
+--                     cases la with
+--                     | leaf =>
+--                         rw [meld.eq_def]
+--                         simp
+--                         exact hrB
+--                     | node lla kla pla rkla rla =>
 
---               sorry
+--                         have lPriority : ¬ pla < pb := by
+--                           rw [not_lt]
+--                           apply le_trans
+--                           . apply hle
+--                           .
+--                             sorry
+--                         simp [lPriority] at hlB
+--                         have bothForAll : forAllHeap p lb ∧ forAllHeap p ((lla.node kla pla rkla rla).meld rb) := by
+--                           apply mkLeftistForAll β p lb ((lla.node kla pla rkla rla).meld rb) kb pb hlB
+--                         exact bothForAll.right
+--                   . intro hRa
+--                     sorry
+--                 . apply leftForAllHeap β p lb rb kb pb rkb hB
+--               . apply forAllHeap.node
+--                 . apply parentPredicate β p lb rb kb pb rkb hB
+--                 . apply leftForAllHeap β p lb rb kb pb rkb hB
+--                 . apply ihRb
+--                   . apply rightForAllHeap β p lb rb kb pb rkb hB
+--                   . intro hLa
 
+--                     sorry
+--                   . intro hRa
+--                     sorry
+
+-- Minheap predicate and lemmas
 inductive minHeap {β : Type} : leftistHeap β → Prop
 | leaf : minHeap leaf
 | node left key priority rank right:
@@ -169,8 +305,15 @@ inductive minHeap {β : Type} : leftistHeap β → Prop
     minHeap right →
     minHeap (node left key priority rank right)
 
-theorem rightMinHeap : ∀ (β : Type) (left right : leftistHeap β) (key : β) (priority : Int) (rank : Nat),
-  minHeap (node left key priority rank right) → minHeap right := by
+
+theorem minHeapLeftForAllHeap : ∀ (β : Type) (left right : leftistHeap β) (key : β) (priority : Int) (rank : Nat),
+  minHeap (node left key priority rank right) → forAllHeap (fun _ pL => priority ≤ pL) left := by
+  intro β left right key priority rank h
+  cases h
+  trivial
+
+theorem minHeapRightForAllHeap : ∀ (β : Type) (left right : leftistHeap β) (key : β) (priority : Int) (rank : Nat),
+  minHeap (node left key priority rank right) → forAllHeap (fun _ pR => priority ≤ pR) right := by
   intro β left right key priority rank h
   cases h
   trivial
@@ -181,22 +324,8 @@ theorem leftMinHeap : ∀ (β : Type) (left right : leftistHeap β) (key : β) (
   cases h
   trivial
 
--- theorem rPriorityLower : ∀ (β : Type) (left rLeft rRight : leftistHeap β) (key rKey: β) (priority rPriority: Int) (rank rRank : Nat),
---   minHeap (node left key priority rank (node rLeft rKey rPriority rRank rRight)) → priority ≤ rPriority := by
---   intro β left rLeft rRight key rKey priority rPriority rank rRank h
---   cases h
-
---   sorry
-
-
-theorem minHeapRightForAllHeap : ∀ (β : Type) (left right : leftistHeap β) (key : β) (priority : Int) (rank : Nat),
-  minHeap (node left key priority rank right) → forAllHeap (fun _ pR => priority ≤ pR) right := by
-  intro β left right key priority rank h
-  cases h
-  trivial
-
-theorem minHeapLeftForAllHeap : ∀ (β : Type) (left right : leftistHeap β) (key : β) (priority : Int) (rank : Nat),
-  minHeap (node left key priority rank right) → forAllHeap (fun _ pL => priority ≤ pL) left := by
+theorem rightMinHeap : ∀ (β : Type) (left right : leftistHeap β) (key : β) (priority : Int) (rank : Nat),
+  minHeap (node left key priority rank right) → minHeap right := by
   intro β left right key priority rank h
   cases h
   trivial
@@ -208,8 +337,11 @@ theorem rightLessThan : ∀ (β : Type) (left right : leftistHeap β) (key : β)
   | leaf => apply forAllHeap.leaf
   | node rLeft rKey rPriority rRank rRight ihL ihR =>
       apply forAllHeap.node
-      .
-        sorry
+      . have lol : forAllHeap (fun _ pR => priority ≤ pR) (node rLeft rKey rPriority rRank rRight) := minHeapRightForAllHeap β left (node rLeft rKey rPriority rRank rRight) key priority rank h
+        have lol' : priority ≤ rPriority := parentPredicate β _ rLeft rRight rKey rPriority rRank lol
+        apply le_trans
+        . apply hPP
+        . apply lol'
       . apply ihL
         apply minHeap.node
         . apply leftForAllHeap β _ left (node rLeft rKey rPriority rRank rRight) key priority rank
@@ -236,15 +368,18 @@ theorem rightLessThan : ∀ (β : Type) (left right : leftistHeap β) (key : β)
         . apply rightMinHeap β rLeft rRight rKey rPriority rRank
           exact rightMinHeap β left _ key priority rank h
 
- theorem leftLessThan : ∀ (β : Type) (left right : leftistHeap β) (key : β) (priority newPriority : Int) (rank : Nat),
+theorem leftLessThan : ∀ (β : Type) (left right : leftistHeap β) (key : β) (priority newPriority : Int) (rank : Nat),
   minHeap (node left key priority rank right) → newPriority ≤ priority → forAllHeap (fun _ pL => newPriority ≤ pL) left := by
   intro β left right key priority newPriority rank h hPP
   induction left with
   | leaf => apply forAllHeap.leaf
   | node lLeft lKey lPriority lRank lRight ihL ihR =>
       apply forAllHeap.node
-      .
-        sorry
+      . have lol : forAllHeap (fun _ pL => priority ≤ pL) (node lLeft lKey lPriority lRank lRight) := minHeapLeftForAllHeap β (node lLeft lKey lPriority lRank lRight) right key priority rank h
+        have lol' : priority ≤ lPriority := parentPredicate β _ lLeft lRight lKey lPriority lRank lol
+        apply le_trans
+        . apply hPP
+        . apply lol'
       . apply ihL
         apply minHeap.node
         . apply leftForAllHeap β _ lLeft lRight lKey lPriority lRank
@@ -264,91 +399,291 @@ theorem rightLessThan : ∀ (β : Type) (left right : leftistHeap β) (key : β)
           exact leftMinHeap β (node lLeft lKey lPriority lRank lRight) right key priority rank h
         . exact rightMinHeap β (node lLeft lKey lPriority lRank lRight) right key priority rank h
 
-structure PriorityQueue (β : Type) where
-  heap : leftistHeap β
-  priority : β → Int
+theorem singleton_minHeap : ∀ (β : Type) (key : β) (priority : Int),
+  minHeap (singleton key priority) := by
+  intro β key priority
+  apply minHeap.node
+  . apply forAllHeap.leaf
+  . apply forAllHeap.leaf
+  . apply minHeap.leaf
+  . apply minHeap.leaf
 
-def newPriorityQueue {β : Type} (priority : β → Int) : PriorityQueue β :=
-  PriorityQueue.mk leftistHeap.leaf priority
+lemma mkLeftistMinHeap : ∀ (β : Type) (left right : leftistHeap β) (key : β) (priority : Int),
+  minHeap (mkLeftistNode left key priority right) → minHeap left ∧ minHeap right := by
+  intro β left right key priority h
+  rw [mkLeftistNode] at h
+  split at h
+  . constructor
+    . exact rightMinHeap β right left key priority ((left.rank) + 1) h
+    . exact leftMinHeap β right left key priority ((left.rank) + 1) h
+  . constructor
+    . exact leftMinHeap β left right key priority ((right.rank) + 1) h
+    . exact rightMinHeap β left right key priority ((right.rank) + 1) h
+
+theorem meld_minHeap : ∀ (β : Type) (a b : leftistHeap β),
+  minHeap a → minHeap b → minHeap (meld a b) := by
+  intro β a b hA hB
+  induction a with
+  | leaf =>
+      rw [meld.eq_def]
+      simp
+      exact hB
+
+  | node la ka pa rka ra ihLa ihRa =>
+      induction b with
+      | leaf =>
+          rw [meld.eq_def]
+          simp
+          exact hA
+
+      | node lb kb pb rkb rb ihLb ihRb =>
+          rw [meld.eq_def]
+          simp
+          split_ifs with hle
+          . rw [mkLeftistNode]
+            split
+            . apply minHeap.node
+              . apply meldForAllHeap
+                . apply minHeapRightForAllHeap β la ra ka pa rka hA
+                . apply forAllHeap.node
+                  . apply le_of_lt hle
+                  . apply leftLessThan β lb rb kb pb pa rkb hB (le_of_lt hle)
+                  . apply rightLessThan β lb rb kb pb pa rkb hB (le_of_lt hle)
+              . apply minHeapLeftForAllHeap β la ra ka pa rka hA
+              . apply ihRa (rightMinHeap β la ra ka pa rka hA)
+              . apply leftMinHeap β la ra ka pa rka hA
+
+            . apply minHeap.node
+              . apply minHeapLeftForAllHeap β la ra ka pa rka hA
+              . apply meldForAllHeap
+                apply minHeapRightForAllHeap β la ra ka pa rka hA
+                apply forAllHeap.node
+                . apply le_of_lt hle
+                . apply leftLessThan β lb rb kb pb pa rkb hB (le_of_lt hle)
+                . apply rightLessThan β lb rb kb pb pa rkb hB (le_of_lt hle)
+              . apply leftMinHeap β la ra ka pa rka hA
+              . apply ihRa (rightMinHeap β la ra ka pa rka hA)
+
+          . rw [mkLeftistNode]
+            rw [not_lt] at hle
+            split
+            . apply minHeap.node
+              . apply meldForAllHeap
+                . apply forAllHeap.node
+                  . apply hle
+                  . apply leftLessThan β la ra ka pa pb rka hA hle
+                  . apply rightLessThan β la ra ka pa pb rka hA hle
+                . apply minHeapRightForAllHeap β lb rb kb pb rkb hB
+              . apply minHeapLeftForAllHeap β lb rb kb pb rkb hB
+              . apply ihRb
+                . apply rightMinHeap β lb rb kb pb rkb hB
+                . intro hLa
+                  have hlab : minHeap (la.meld (lb.node kb pb rkb rb)) := by apply ihLa hLa
+                  have hrB : minHeap rb := by apply rightMinHeap β lb rb kb pb rkb hB
+                  rw [meld.eq_def] at hlab
+                  cases la with
+                  | leaf =>
+                      rw [meld.eq_def]
+                      simp
+                      exact hrB
+                  | node lla kla pla rkla rla =>
+                      have lPriority : ¬ pla < pb := by
+                        rw [not_lt]
+                        apply le_trans
+                        . apply hle
+                        . have lol : forAllHeap (fun _ pL => pa ≤ pL) (node lla kla pla rkla rla) := by
+                            apply minHeapLeftForAllHeap β (node lla kla pla rkla rla) ra ka pa rka hA
+                          apply parentPredicate β _ lla rla kla pla rkla lol
+                      simp [lPriority] at hlab
+                      have bothForAll : minHeap lb ∧ minHeap ((lla.node kla pla rkla rla).meld rb) := by
+                        apply mkLeftistMinHeap β lb ((lla.node kla pla rkla rla).meld rb) kb pb hlab
+                      exact bothForAll.right
+
+                . intro hRa
+                  have hrab : minHeap (ra.meld (lb.node kb pb rkb rb)) := by apply ihRa hRa
+                  have hrB : minHeap rb := by apply rightMinHeap β lb rb kb pb rkb hB
+                  rw [meld.eq_def] at hrab
+                  cases ra with
+                  | leaf =>
+                      rw [meld.eq_def]
+                      simp
+                      exact hrB
+                  | node lra kra pra rkra rra =>
+                      have rPriority : ¬ pra < pb := by
+                        rw [not_lt]
+                        apply le_trans
+                        . apply hle
+                        . have lol : forAllHeap (fun _ pL => pa ≤ pL) (node lra kra pra rkra rra) := by
+                            apply minHeapRightForAllHeap β la (node lra kra pra rkra rra) ka pa rka hA
+                          apply parentPredicate β _ lra rra kra pra rkra lol
+                      simp [rPriority] at hrab
+                      have bothForAll : minHeap lb ∧ minHeap ((node lra kra pra rkra rra).meld rb) := by
+                        apply mkLeftistMinHeap β lb ((node lra kra pra rkra rra).meld rb) kb pb hrab
+                      exact bothForAll.right
+
+              . apply leftMinHeap β lb rb kb pb rkb hB
+
+            . apply minHeap.node
+              . apply minHeapLeftForAllHeap β lb rb kb pb rkb hB
+              . apply meldForAllHeap
+                . apply forAllHeap.node
+                  . apply hle
+                  . apply leftLessThan β la ra ka pa pb rka hA hle
+                  . apply rightLessThan β la ra ka pa pb rka hA hle
+                . apply minHeapRightForAllHeap β lb rb kb pb rkb hB
+              . apply leftMinHeap β lb rb kb pb rkb hB
+              . apply ihRb
+                . apply rightMinHeap β lb rb kb pb rkb hB
+                . intro hLa
+                  have hlab : minHeap (la.meld (lb.node kb pb rkb rb)) := by apply ihLa hLa
+                  have hrB : minHeap rb := by apply rightMinHeap β lb rb kb pb rkb hB
+                  rw [meld.eq_def] at hlab
+                  cases la with
+                  | leaf =>
+                      rw [meld.eq_def]
+                      simp
+                      exact hrB
+                  | node lla kla pla rkla rla =>
+                      have lPriority : ¬ pla < pb := by
+                        rw [not_lt]
+                        apply le_trans
+                        . apply hle
+                        . have lol : forAllHeap (fun _ pL => pa ≤ pL) (node lla kla pla rkla rla) := by
+                            apply minHeapLeftForAllHeap β (node lla kla pla rkla rla) ra ka pa rka hA
+                          apply parentPredicate β _ lla rla kla pla rkla lol
+                      simp [lPriority] at hlab
+                      have bothForAll : minHeap lb ∧ minHeap ((lla.node kla pla rkla rla).meld rb) := by
+                        apply mkLeftistMinHeap β lb ((lla.node kla pla rkla rla).meld rb) kb pb hlab
+                      exact bothForAll.right
+
+                . intro hRa
+                  have hrab : minHeap (ra.meld (lb.node kb pb rkb rb)) := by apply ihRa hRa
+                  have hrB : minHeap rb := by apply rightMinHeap β lb rb kb pb rkb hB
+                  rw [meld.eq_def] at hrab
+                  cases ra with
+                  | leaf =>
+                      rw [meld.eq_def]
+                      simp
+                      exact hrB
+                  | node lra kra pra rkra rra =>
+                      have rPriority : ¬ pra < pb := by
+                        rw [not_lt]
+                        apply le_trans
+                        . apply hle
+                        . have lol : forAllHeap (fun _ pL => pa ≤ pL) (node lra kra pra rkra rra) := by
+                            apply minHeapRightForAllHeap β la (node lra kra pra rkra rra) ka pa rka hA
+                          apply parentPredicate β _ lra rra kra pra rkra lol
+                      simp [rPriority] at hrab
+                      have bothForAll : minHeap lb ∧ minHeap ((node lra kra pra rkra rra).meld rb) := by
+                        apply mkLeftistMinHeap β lb ((node lra kra pra rkra rra).meld rb) kb pb hrab
+                      exact bothForAll.right
+
+structure PriorityQueue (β : Type) where
+  heap : leftistHeap β -- the heap structure containing the elements
+  p : β → Int -- the priority function that assigns a priority to each element
+
+def newPriorityQueue {β : Type} (p : β → Int) : PriorityQueue β :=
+  PriorityQueue.mk leftistHeap.leaf p
 
 def insertPQ {β : Type} (pq : PriorityQueue β) (key : β) : PriorityQueue β :=
-  PriorityQueue.mk (leftistHeap.insertLeftist pq.heap key (pq.priority key)) pq.priority
+  PriorityQueue.mk (leftistHeap.insertLeftist pq.heap key (pq.p key)) pq.p
 
-def deleteMin {β : Type} (pq : PriorityQueue β) : Option (β × Int) × PriorityQueue β :=
+def deleteMinPQ {β : Type} (pq : PriorityQueue β) : Option (β × Int) × PriorityQueue β :=
   match pq.heap with
   | leftistHeap.leaf => ⟨none, pq⟩
   | leftistHeap.node left key priority _ right =>
-    ⟨(key, priority), PriorityQueue.mk (leftistHeap.meld left right) pq.priority⟩
+    ⟨(key, priority), PriorityQueue.mk (leftistHeap.meld left right) pq.p⟩
 
-theorem insert_minHeap : ∀ (β : Type) (p : β → Int → Prop) (h : leftistHeap β) (newKey : β) (newPriority : Int),
+-- theorem insert_minHeap_old : ∀ (β : Type)  (h : leftistHeap β) (newKey : β) (newPriority : Int),
+--   minHeap h → minHeap (insertLeftist h newKey newPriority) := by
+--     intro β h newKey newPriority hP
+--     induction h with
+--     | leaf =>
+--         rw [insertLeftist, meld, singleton]
+--         apply minHeap.node
+--         apply forAllHeap.leaf
+--         apply forAllHeap.leaf
+--         apply minHeap.leaf
+--         apply minHeap.leaf
+
+--     | node left key priority rank right ihL ihR =>
+--         rw [insertLeftist, meld.eq_def, singleton]
+--         simp
+--         split
+
+--         case isTrue hPP =>
+--           rw [mkLeftistNode]
+--           split
+
+--           case isTrue =>
+--             apply minHeap.node
+--             . rw [insertLeftist, singleton] at ihR
+--               apply forAllHeap_insertLeftist _ _ _
+--               apply minHeapRightForAllHeap β left right key priority rank hP
+--               apply Int.le_of_lt hPP
+--             . exact minHeapLeftForAllHeap β left right key priority rank hP
+--             . apply ihR
+--               exact rightMinHeap β left right key priority rank hP
+--             . exact leftMinHeap β left right key priority rank hP
+
+--           case isFalse =>
+--             apply minHeap.node
+--             . apply minHeapLeftForAllHeap β left right key priority rank hP
+--             . rw [insertLeftist, singleton] at ihR
+--               apply forAllHeap_insertLeftist _ _ _
+--               apply minHeapRightForAllHeap β left right key priority rank hP
+--               apply Int.le_of_lt hPP
+--             . exact leftMinHeap β left right key priority rank hP
+--             . apply ihR
+--               exact rightMinHeap β left right key priority rank hP
+
+--         case isFalse hPP =>
+--           rw [mkLeftistNode]
+--           rw [Int.not_lt] at hPP
+--           split
+--           case isTrue =>
+--             rw [meld.eq_def]
+--             simp
+--             apply minHeap.node
+--             apply forAllHeap.node
+--             apply hPP
+--             apply leftLessThan β left right key priority newPriority rank hP hPP
+--             apply rightLessThan β left right key priority newPriority rank hP hPP
+--             apply forAllHeap.leaf
+--             apply hP
+--             apply minHeap.leaf
+--           case isFalse =>
+--             rw [meld.eq_def]
+--             simp
+--             apply minHeap.node
+--             apply forAllHeap.leaf
+--             apply forAllHeap.node
+--             apply hPP
+--             apply leftLessThan β left right key priority newPriority rank hP hPP
+--             apply rightLessThan β left right key priority newPriority rank hP hPP
+--             apply minHeap.leaf
+--             apply hP
+
+theorem insertLeftist_correct : ∀ (β : Type)  (h : leftistHeap β) (newKey : β) (newPriority : Int),
   minHeap h → minHeap (insertLeftist h newKey newPriority) := by
-    intro β p h newKey newPriority hP
-    induction h with
-    | leaf =>
-        rw [insertLeftist, meld, singleton]
-        apply minHeap.node
-        apply forAllHeap.leaf
-        apply forAllHeap.leaf
-        apply minHeap.leaf
-        apply minHeap.leaf
+  intro β h newKey newPriority hP
+  induction h with
+  | leaf =>
+      rw [insertLeftist, singleton]
+      apply meld_minHeap
+      . apply minHeap.leaf
+      . apply singleton_minHeap
+  | node left key priority rank right ihL ihR =>
+      rw [insertLeftist]
+      apply meld_minHeap
+      . exact hP
+      . apply singleton_minHeap
 
-    | node left key priority rank right ihL ihR =>
-        rw [insertLeftist, meld.eq_def, singleton]
-        simp
-        split
-
-        case isTrue hPP =>
-          rw [mkLeftistNode]
-          split
-
-          case isTrue =>
-            apply minHeap.node
-            . rw [insertLeftist, singleton] at ihR
-              apply forAllHeap_insertLeftist _ _ _
-              apply minHeapRightForAllHeap β left right key priority rank hP
-              apply Int.le_of_lt hPP
-            . exact minHeapLeftForAllHeap β left right key priority rank hP
-            . apply ihR
-              exact rightMinHeap β left right key priority rank hP
-            . exact leftMinHeap β left right key priority rank hP
-
-          case isFalse =>
-            apply minHeap.node
-            . apply minHeapLeftForAllHeap β left right key priority rank hP
-            . rw [insertLeftist, singleton] at ihR
-              apply forAllHeap_insertLeftist _ _ _
-              apply minHeapRightForAllHeap β left right key priority rank hP
-              apply Int.le_of_lt hPP
-            . exact leftMinHeap β left right key priority rank hP
-            . apply ihR
-              exact rightMinHeap β left right key priority rank hP
-
-        case isFalse hPP =>
-          rw [mkLeftistNode]
-          rw [Int.not_lt] at hPP
-          split
-          case isTrue =>
-            rw [meld.eq_def]
-            simp
-            apply minHeap.node
-            apply forAllHeap.node
-            apply hPP
-            apply leftLessThan β left right key priority newPriority rank hP hPP
-            apply rightLessThan β left right key priority newPriority rank hP hPP
-            apply forAllHeap.leaf
-            apply hP
-            apply minHeap.leaf
-          case isFalse =>
-            rw [meld.eq_def]
-            simp
-            apply minHeap.node
-            apply forAllHeap.leaf
-            apply forAllHeap.node
-            apply hPP
-            apply leftLessThan β left right key priority newPriority rank hP hPP
-            apply rightLessThan β left right key priority newPriority rank hP hPP
-            apply minHeap.leaf
-            apply hP
-
+theorem deleteMin_correct : ∀ (β : Type) (pq : PriorityQueue β),
+  minHeap pq.heap → ∀ (key : β) (priority : Int), pq.p key = priority → minHeap (insertLeftist pq.heap key priority) := by
+  intro β pq hP key priority hKey
+  rw [insertLeftist]
+  apply insertLeftist_correct
+  exact hP
 
 end leftistHeap
